demo/fib/Fib01proof.v
@@ -18,8 +18,236 @@ Require Import Clightdefs Op ClightC CtypesC CtypingC.
 Require Import FibHeader.
 Require Import Fib1.
 Require Import Fib0.
+Require Import SIRUnstackproof.
 
 Set Implicit Arguments.
+
+(*** TODO: copied from unstackproof. move to coqlibc ***)
+Tactic Notation "substs" :=
+  repeat (match goal with H: ?x = ?y |- _ =>
+            first [ subst x | subst y ] end).
+
+Notation "'_'" := PTree.Leaf (at level 150).
+Notation "a % x % b" := (PTree.Node a x b) (at level 150).
+Notation "a %% b" := (PTree.Node a None b) (at level 150).
+
+(*** TODO: remove redundancy with unstackproof ***)
+Notation "'geof'" :=
+  (fun skenv_link p_tgt =>
+     Build_genv (SkEnv.revive ((SkEnv.project skenv_link)
+                                 (CSk.of_program signature_of_function p_tgt)) p_tgt)
+                (p_tgt.(prog_comp_env))) (at level 50).
+
+(* Local Opaque PTree.get. *)
+Opaque _fib.
+Theorem correct: rusc defaultR [Fib1.module: Mod.t] [Fib0.module: Mod.t].
+Proof.
+  eapply SIRUnstackproof.correct; ss; et.
+  econs; ss; et.
+  - ii. u. des_ifs. unfold internal_funs. des_ifs. exploit prog_defmap_image; et. ss. ii; des; ss.
+  - ii.
+    assert(INCL: SkEnv.includes skenv_link (Mod.sk Fib0.module)).
+    { admit "ez". }
+    (*** THIS SHOULD BE PROVIDED FROM META THEORY ***)
+    assert(exists fblk, <<SYMB: Genv.find_symbol (geof skenv_link prog) _fib = Some fblk>>).
+    {
+      inv INCL. ss.
+      exploit (DEFS _fib); et.
+      { unfold prog_defmap. ss. }
+      i; des. ss. folder.
+      clear - SYMB.
+      Local Opaque PTree.get.
+      (*** TODO: Current: I can't use global opaque because of some extensional proofs. fix it ***)
+      uge. ss. rewrite MapsC.PTree_filter_key_spec. des_ifs. esplits; et.
+      Local Transparent PTree.get.
+    }
+    des.
+    (*** THIS SHOULD BE PROVIDED FROM META THEORY ***)
+    assert(FIBDEF: forall
+              fblk
+              (SYMB: Genv.find_symbol (geof skenv_link prog) _fib = Some fblk)
+            ,
+              <<DEF: Genv.find_funct (geof skenv_link prog) (Vptr fblk Ptrofs.zero)
+                     = Some (Ctypes.Internal f_fib)>>).
+    { i.
+      exploit (SkEnv.project_impl_spec); try apply INCL. intro SPEC.
+      des. ss. des_ifs. clear_tac.
+      exploit CSkEnv.project_revive_precise; et. intro T. inv T.
+      exploit SYMB2P; et. intro U. dup U. unfold NW, defs in U0. des_sumbool.
+      exploit prog_defmap_dom; et. intro V; des.
+      exploit P2GE; et. intro W; des.
+      folder.
+      assert(fblk = b).
+      { clear - SPEC SYMB SYMB0 U. (*** TODO: this is too extensional ***) uge. ss. clarify. }
+      clarify.
+      exploit (prog_defmap_norepet prog _fib); ss; et.
+      { repeat (econs; ss; et; [ii; des; ss|]); repeat econs; ss; et. }
+      intro T. clarify. ss.
+      unfold Genv.find_funct_ptr. unfold Clight.fundef. rewrite DEF. ss.
+    }
+    exploit FIBDEF; et. intro DEF. clear FIBDEF.
+    des.
+
+
+    exploit prog_defmap_image; et. ss. ii; des; ss. clarify.
+    exploit (prog_defmap_norepet prog _fib); et.
+    { repeat (econs; ss; et). }
+    { ss; et. }
+    ii; clarify. cbn in SRC. des_ifs. clear_tac.
+    econs; ss; et. ii. inv TYP. ss. destruct vs0; ss. destruct vs0; ss. cbn in TYP0. clarify.
+    clear_tac.
+
+    esplits; et.
+    { repeat (econs; ss; et).
+      ii; ss; try (by repeat des; ss; clarify).
+    }
+    assert(exists n, v = Vint n).
+    { admit "stronger typecheck (not allowing undef)". }
+    des. clarify. clear H0.
+    destruct (classic (Int.eq n Int.zero)).
+    { apply_all_once Int.same_if_eq. clarify.
+      pfold. econs; ss; et; cycle 1.
+      { eapply plus_left with (t1 := E0) (t2 := E0); ss.
+        { _step. }
+        eapply star_left with (t1 := E0) (t2 := E0); ss.
+        { _step. }
+        des_ifs.
+        eapply star_left with (t1 := E0) (t2 := E0); ss.
+        { _step. }
+        apply star_refl.
+      }
+      { des_ifs. left. pfold. econs; ss; et. }
+    }
+    rename H into NZERO.
+    destruct (classic (Int.eq n Int.one)).
+    { apply_all_once Int.same_if_eq. clarify.
+      pfold. econs; ss; et; cycle 1.
+      { eapply plus_left with (t1 := E0) (t2 := E0); ss.
+        { _step. }
+        eapply star_left with (t1 := E0) (t2 := E0); ss.
+        { _step. }
+        des_ifs.
+        eapply star_left with (t1 := E0) (t2 := E0); ss.
+        { _step. }
+        eapply star_left with (t1 := E0) (t2 := E0); ss.
+        { _step. }
+        eapply star_left with (t1 := E0) (t2 := E0); ss.
+        { _step. }
+        eapply star_left with (t1 := E0) (t2 := E0); ss.
+        { _step. }
+        apply star_refl.
+      }
+      { des_ifs. left. pfold. econs; ss; et. }
+    }
+    rename H into NONE.
+
+    {
+      pfold. econs; ss; et; cycle 1.
+      { eapply plus_left with (t1 := E0) (t2 := E0); ss.
+        { _step. }
+        eapply star_left with (t1 := E0) (t2 := E0); ss.
+        { repeat (econs; ss; et). ss. rewrite Int.eq_false; ss. ii; clarify. }
+        eapply star_left with (t1 := E0) (t2 := E0); ss.
+        { _step. }
+        eapply star_left with (t1 := E0) (t2 := E0); ss.
+        { _step. }
+        eapply star_left with (t1 := E0) (t2 := E0); ss.
+        { repeat (econs; ss; et). ss. rewrite Int.eq_false; ss. ii; clarify. }
+        eapply star_left with (t1 := E0) (t2 := E0); ss.
+        { _step. }
+        eapply star_left with (t1 := E0) (t2 := E0); ss.
+        { _step. }
+        eapply star_left with (t1 := E0) (t2 := E0); ss.
+        { _step. }
+        eapply star_left with (t1 := E0) (t2 := E0); ss.
+        { _step. }
+        apply star_refl.
+      }
+      des_ifs. rewrite bind_trigger.
+      left. pfold. econs; ss; et.
+      { econs; ss; et. cbn. unfold typify. des_ifs; ss. }
+      ii.
+      left. pfold. econs; ss; et; cycle 1.
+      { eapply plus_left with (t1 := E0) (t2 := E0); ss.
+        { _step. }
+        eapply star_left with (t1 := E0) (t2 := E0); ss.
+        { _step. }
+        eapply star_left with (t1 := E0) (t2 := E0); ss.
+        { _step. }
+        eapply star_left with (t1 := E0) (t2 := E0); ss.
+        { _step. }
+        eapply star_left with (t1 := E0) (t2 := E0); ss.
+        { _step. }
+        eapply star_left with (t1 := E0) (t2 := E0); ss.
+        { _step. }
+        apply star_refl.
+      }
+      left. pfold.
+      rewrite bind_trigger.
+      econs; ss; et.
+      { econs; ss; et. cbn. unfold typify. des_ifs; ss. }
+      ii.
+      left. pfold. econs; ss; et; cycle 1.
+      { eapply plus_left with (t1 := E0) (t2 := E0); ss.
+        { _step. }
+        eapply star_left with (t1 := E0) (t2 := E0); ss.
+        { _step. }
+        eapply star_left with (t1 := E0) (t2 := E0); ss.
+        { _step. }
+        eapply star_left with (t1 := E0) (t2 := E0); ss.
+        { repeat (econs; ss; et).
+          -
+          - }
+        eapply star_left with (t1 := E0) (t2 := E0); ss.
+        { _step. }
+        eapply star_left with (t1 := E0) (t2 := E0); ss.
+        { _step. }
+        apply star_refl.
+      }
+      {
+      { left. pfold. econs; ss; et. des_ifs; et. unfold Genv.find_funct_ptr.
+
+      step.
+      eapply star_left with (t1 := E0) (t2 := E0); ss.
+      { repeat (econs; ss; et). ss. rewrite Int.eq_false; ss. ii; clarify. }
+      step. ss. apply star_refl.
+      }
+      { des_ifs. left. pfold. econs; ss; et. }
+    }
+
+
+    destruct (classic (Int.eq n Int.one)).
+    { apply_all_once Int.same_if_eq. clarify.
+      eexists _, _, (SimMemId.mk _ _). esplits; eauto.
+      { left. eapply spread_dplus; et.
+        { eapply modsem2_mi_determinate; et. }
+        step. ss. apply star_refl.
+      }
+      { right. eapply CIH.
+        econs; ss; et. econs; ss; et.
+      }
+    }
+    rename H into NONE.
+
+
+    esplits; et.
+    { repeat (econs; ss; et).
+      ii; ss; try (by repeat des; ss; clarify).
+    }
+    pfold. econs; ss; et; cycle 1.
+    { eapply plus_left with (t1 := E0) (t2 := E0); ss.
+      { _step. }
+
+
+      eapply star_left with (t1 := E0) (t2 := E0); ss.
+      { repeat (econs; ss; et).
+        - ss. rewrite Int.eq_false; ss. ii; clarify. }
+        econs; ss; et. _step.
+      }
+    }
+Unshelve.
+  sk_incl_tac.
+Qed.
 
 Program Instance SMO: SimMemOh.class := (SimMemOh_default_aux _ (Some "fib")).
 Local Arguments ModSemPair.mk [SM] [SS] _ _ _ _ [SMO].
